aaa

queue.dfy
@@ -1,15 +1,69 @@
 
 class Queue {
+    var list: array<int>;
+    var size: int;
+    var first: int;
 
-    constructor() {}
+    ghost var list_ghost: array<int>;
+    ghost var size_ghost: int;
 
-    method push() {}
+    // Invariant: size is non-negative
+    // Invariant: size is less than or equal to the length of list
+    // Invariant: all elements of list before index size are valid
+    // Invariant: all elements of list after index size are zero
+    predicate Valid()
+        reads *
+    {
+        0 <= size <= list.Length
+        // forall i :: 0 <= i < size ==> list[i] |-> ? &&
+        // forall i :: size <= i < list.Length ==> list[i] == 0
+    }
+
+    constructor()
+        ensures Valid()
+    {
+        list := new int[100];
+        size := 0;
+        first := 0;
+    }
+
+    method enqueue(x: int)
+        requires Valid()
+        // ensures size_ghost == old(size_ghost) + 1
+        // ensures list_ghost[size_ghost - 1] == x
+        ensures Valid()
+        modifies list, this
+    {
+        list[size] := x;
+        size := size + 1;
+
+    }
+
+    method grow() 
+        requires Valid()
+        ensures list.Length == 2 * old(list.Length)
+        modifies this
+    {
+        var new_list := new int[list.Length * 2];
+
+        var i := 0;
+        while (i < size) 
+            invariant i >= 0;
+            invariant i <= size;
+            decreases size - i;
+        {
+            new_list[i] := list[i];
+            i := i + 1;
+        }
+
+        list := new_list;
+    }
 
     method pop() {}
 
     method contains() {}
 
-    method size() {}
+    method length() {}
 
     method isEmpty() {}
 
